Make reactor state a list instead of vector.

src/determinism.lean
@@ -3,24 +3,24 @@ import data.vector
 
 namespace hidden 
 
-  variables i o s : ℕ 
+  variables i o : ℕ 
 
   def inputs := vector value i
   def outputs := vector value o
-  def state := vector value s
+  def state := list value
 
   -- REACTION
 
   -- The output vector produced by a reaction contains ε for all of those ports which should remain unaffected.
-  def reaction := (inputs i × state s) → (outputs o × state s)
+  def reaction := (inputs i × state) → (outputs o × state)
   
   namespace reaction
 
-    def determinism {i o s : ℕ} (r : reaction i o s) : Prop := 
-      ∀ is₁ is₂ : (inputs i × state s), is₁ = is₂ → r is₁ = r is₂
+    def determinism {i o : ℕ} (r : reaction i o) : Prop := 
+      ∀ is₁ is₂ : (inputs i × state), is₁ = is₂ → r is₁ = r is₂
 
-    theorem deterministic (r : reaction i o s) : determinism r :=
-      assume is₁ is₂ : (inputs i × state s),
+    theorem deterministic (r : reaction i o) : determinism r :=
+      assume is₁ is₂ : (inputs i × state),
       assume h : is₁ = is₂,
       show r is₁ = r is₂,
       from congr_arg r h
@@ -31,26 +31,26 @@ namespace hidden
 
   -- The order produced by a body only describes the *priority* of the reactions, not their connections.
   inductive body
-    | single (r : reaction i o s) : body
-    | composed (head : reaction i o s) (tail : body) : body
+    | single (r : reaction i o) : body
+    | composed (head : reaction i o) (tail : body) : body
 
   namespace body
 
     private def merge {o : ℕ} (o₁ o₂ : outputs o) : outputs o := sorry
 
-    private def process' {i o s : ℕ} : (inputs i × outputs o × state s) → (body i o s) → (outputs o × state s)
+    private def process' {i o : ℕ} : (inputs i × outputs o × state) → (body i o) → (outputs o × state)
       | ios (body.single r)     := let os := r ⟨ios.1, ios.2.2⟩ in ⟨merge os.1 ios.2.1, os.2⟩ 
       | ios (body.composed r t) := let os := r ⟨ios.1, ios.2.2⟩ in let os' := process' ⟨ios.1, os.1, os.2⟩ t in ⟨merge os.1 os'.1, os'.2⟩ 
 
-    def process {i o s : ℕ} : (inputs i × state s) → (body i o s) → (outputs o × state s)
+    def process {i o : ℕ} : (inputs i × state) → (body i o) → (outputs o × state)
       | is (body.single r)     := r is
       | is (body.composed r t) := let os := r is in process' ⟨is.1, os.1, os.2⟩ t
 
-    def determinism {i o s : ℕ} (b : body i o s) : Prop := 
-      ∀ is₁ is₂ : (inputs i × state s), is₁ = is₂ → (process is₁ b) = (process is₂ b)
+    def determinism {i o : ℕ} (b : body i o) : Prop := 
+      ∀ is₁ is₂ : (inputs i × state), is₁ = is₂ → (process is₁ b) = (process is₂ b)
 
-    theorem deterministic (b : body i o s) : determinism b :=
-      assume is₁ is₂ : (inputs i × state s),
+    theorem deterministic (b : body i o) : determinism b :=
+      assume is₁ is₂ : (inputs i × state),
       assume h : is₁ = is₂,
       show process is₁ b = process is₂ b,
       from congr (congr_arg process h) (refl b)
@@ -62,17 +62,17 @@ namespace hidden
   namespace sequence
     
     -- Given a list of inputs, an initial state and a body, `process` computes the resulting state and outputs.
-    def process {i o s : ℕ} : list (inputs i) → (state s) → (body i o s) → list (outputs o × state s)
+    def process {i o : ℕ} : list (inputs i) → (state) → (body i o) → list (outputs o × state)
       | [] _ _ := []
       | (list.cons i_h i_t) s b := let os' := body.process ⟨i_h, s⟩ b in list.cons os' (process i_t os'.2 b) 
 
-    def determinism {i o s : ℕ} (b : body i o s) : Prop := 
-      ∀ (i₁ i₂ : list (inputs i)) (s₁ s₂ : state s), 
+    def determinism {i o : ℕ} (b : body i o) : Prop := 
+      ∀ (i₁ i₂ : list (inputs i)) (s₁ s₂ : state), 
       (i₁ = i₂ ∧ s₁ = s₂) → (process i₁ s₁ b) = (process i₂ s₂ b)
 
-    theorem deterministic (b : body i o s) : determinism b :=
+    theorem deterministic (b : body i o) : determinism b :=
       assume i₁ i₂ : list (inputs i),
-      assume s₁ s₂ : state s,
+      assume s₁ s₂ : state,
       assume h : i₁ = i₂ ∧ s₁ = s₂,
       show process i₁ s₁ b = process i₂ s₂ b, 
       from congr (congr (congr_arg process h.left) h.right) (refl b)
@@ -84,17 +84,17 @@ namespace hidden
   structure reactor :=
     (in_ports : inputs i)
     (out_ports : outputs o)
-    (st : state s)
-    (b : body i o s)
+    (s : state)
+    (b : body i o)
 
   -- NETWORK
 
   -- By defining the `reactors` as a list instead of a set, we can again drop the need for identifiers and use the index
   -- into the list as a reactor's identifier.
   --
-  -- The list needs to be homogenous over the type of rectors wrt. `i o s`. Is this possible?
+  -- The list needs to be homogenous over the type of rectors wrt. `i o`. Is this possible?
   structure network :=
-    (reactors : list (reactor i o s))
-    (connections : (reactor i o s) × ℕ → (reactor i o s) × ℕ)
+    (reactors : list (reactor i o))
+    (connections : (reactor i o) × ℕ → (reactor i o) × ℕ)
 
 end hidden
